Setlec/Verify/Fueled.lean
@@ -289,6 +289,15 @@ theorem projCert_atF (d : Nat) (lic : Bool) (c : Name) (us : List Level)
   · exact iotaCerts_atF d lic F _ _
   · rfl
 
+theorem projCertAt_atF (d : Nat) (v lic : Bool) (c : Name) (us : List Level)
+    (args : List Expr) (F : Nat) :
+    (projCertAt (fueledFns mode env) env d v lic c us args).val F =
+      projCertAt (pureFns mode env F) env d v lic c us args := by
+  unfold projCertAt
+  split
+  · exact projCert_atF d lic c us args F
+  · rfl
+
 macro "atF_step2" : tactic =>
   `(tactic| repeat (first
     | rfl
@@ -304,6 +313,7 @@ macro "atF_step2" : tactic =>
     | (rw [structEtaCertWith_atF])
     | (rw [structUnitCert_atF])
     | (rw [etaCert_atF])
+    | (rw [projCertAt_atF])
     | (rw [projCert_atF])
     | ((rw [FueledM.atF_bind]; congr 1 <;> try rfl) <;> try funext _)
     | (dsimp only [])
@@ -393,6 +403,7 @@ macro "atF_step3" : tactic =>
     | (rw [structEtaCertWith_atF])
     | (rw [structUnitCert_atF])
     | (rw [etaCert_atF])
+    | (rw [projCertAt_atF])
     | (rw [projCert_atF])
     | (rw [structEtaCert_atF])
     | (rw [majorToCtor_atF])
@@ -438,6 +449,7 @@ macro "atF_core4" x:tactic : tactic =>
     | (rw [structEtaCertWith_atF])
     | (rw [structUnitCert_atF])
     | (rw [etaCert_atF])
+    | (rw [projCertAt_atF])
     | (rw [projCert_atF])
     | (rw [structEtaCert_atF])
     | (rw [majorToCtor_atF])
